Implemented product machine

Adaptive_State_Counting/FSM/FSM3.thy
@@ -2,40 +2,43 @@ theory FSM3
 imports Main
 begin
 
-type_synonym State = nat
+(*type_synonym State = nat*)
 type_synonym Input = nat
 type_synonym Output = nat
-type_synonym Transition = "(nat \<times> nat \<times> nat \<times> nat)"
+(*type_synonym Transition = "(nat \<times> nat \<times> nat \<times> nat)"*)
+type_synonym 'state Transition = "('state \<times> Input \<times> Output \<times> 'state)"
 
-record FSM = 
-  initial :: State 
+record 'state FSM = 
+  initial :: 'state 
   inputs  :: "Input list"
   outputs  :: "Output list"  
-  transitions :: "Transition list" 
+  transitions :: "('state Transition) list" 
 
-abbreviation "t_source (a :: Transition) \<equiv> fst a" 
-abbreviation "t_input  (a :: Transition) \<equiv> fst (snd a)"
-abbreviation "t_output (a :: Transition) \<equiv> fst (snd (snd a))"
-abbreviation "t_target (a :: Transition) \<equiv> snd (snd (snd a))"
+abbreviation "t_source (a :: 'state Transition) \<equiv> fst a" 
+abbreviation "t_input  (a :: 'state Transition) \<equiv> fst (snd a)"
+abbreviation "t_output (a :: 'state Transition) \<equiv> fst (snd (snd a))"
+abbreviation "t_target (a :: 'state Transition) \<equiv> snd (snd (snd a))"
 
-value "t_source (1,2,3,4)"
-value "t_input  (1,2,3,4)"
-value "t_output (1,2,3,4)"
-value "t_target (1,2,3,4)"
+abbreviation "p_io (p :: 'state Transition list) \<equiv> map (\<lambda> t . (t_input t, t_output t)) p"
+
+value "t_source (1,2,3,4::nat)"
+value "t_input  (1,2,3,4::nat)"
+value "t_output (1,2,3,4::nat)"
+value "t_target (1,2,3,4::nat)"
 
 
 
-fun is_wf_transition :: "FSM \<Rightarrow> Transition \<Rightarrow> bool" where
+fun is_wf_transition :: "'state FSM \<Rightarrow> 'state Transition \<Rightarrow> bool" where
   "is_wf_transition M t = ((t_input t) \<in> set (inputs M) \<and> (t_output t) \<in> set (outputs M))"
 
-fun wf_transitions :: "FSM \<Rightarrow> Transition list" where
+fun wf_transitions :: "'state FSM \<Rightarrow> 'state Transition list" where
   "wf_transitions M = filter (is_wf_transition M) (transitions M)"
 
 abbreviation "h M \<equiv> set (wf_transitions M)"
 
 
 
-fun pairwise_immediately_reachable :: "FSM \<Rightarrow> (State \<times> State) set" where
+fun pairwise_immediately_reachable :: "'state FSM \<Rightarrow> ('state  \<times> 'state ) set" where
   "pairwise_immediately_reachable M =  image (\<lambda> t. (t_source t, t_target t)) (h M)"
 
 lemma wf_transrel_transition_ob : 
@@ -47,16 +50,16 @@ lemma wf_transrel_transition_ob :
     and "is_wf_transition M t"
   using assms by auto
 
-fun pairwise_reachable :: "FSM \<Rightarrow> (State \<times> State) set" where
+fun pairwise_reachable :: "'state FSM \<Rightarrow> ('state  \<times> 'state ) set" where
   "pairwise_reachable M = trancl (pairwise_immediately_reachable M)"
 
-fun reachable :: "FSM \<Rightarrow> State \<Rightarrow> State \<Rightarrow> bool" where
+fun reachable :: "'state FSM \<Rightarrow> 'state \<Rightarrow> 'state \<Rightarrow> bool" where
   "reachable M q q' = (q = q' \<or> (q, q') \<in> pairwise_reachable M)"
 
-fun initially_reachable :: "FSM \<Rightarrow> State \<Rightarrow> bool" where
+fun initially_reachable :: "'state FSM \<Rightarrow> 'state \<Rightarrow> bool" where
   "initially_reachable M q = reachable M (initial M) q"
 
-fun nodes :: "FSM \<Rightarrow> State set" where
+fun nodes :: "'state FSM \<Rightarrow> 'state set" where
   "nodes M = insert (initial M) (set (filter (initially_reachable M) (map t_target (wf_transitions M))))"
 
 
@@ -73,7 +76,7 @@ proof -
   proof (cases "q = t_source t")
     case True
     then show ?thesis
-      using \<open>(t_source t, t_target t) \<in> pairwise_reachable M\<close> reachable.simps by blast 
+      using \<open>(t_source t, t_target t) \<in> pairwise_reachable M\<close> by auto       
   next
     case False
     then have "(q, t_source t) \<in> pairwise_reachable M" 
@@ -109,9 +112,24 @@ next
     using assms(2) by auto
 qed
 
-fun path :: "FSM \<Rightarrow> State \<Rightarrow> Transition list \<Rightarrow> bool" where
-  "path M q [] = True" |
-  "path M q (t#ts) = (t \<in> h M \<and> q = t_source t \<and> path M (t_target t) ts)"
+
+
+
+inductive path :: "'state FSM \<Rightarrow> 'state \<Rightarrow> 'state Transition list \<Rightarrow> bool" where
+  nil[intro!] : "path M q []" |
+  cons[intro!] : "t \<in> h M \<Longrightarrow> path M (t_target t) ts \<Longrightarrow> path M (t_source t) (t#ts)"
+
+inductive_cases path_cons_elim[elim!]: "path M q (t#ts)"
+
+
+fun path' :: "'state FSM \<Rightarrow> 'state \<Rightarrow> 'state Transition list \<Rightarrow> bool" where
+  "path' M q [] = True" |
+  "path' M q (t#ts) = (t \<in> h M \<and> q = t_source t \<and> path M (t_target t) ts)"
+
+
+lemma path_code[code] : "path M q p = path' M q p" 
+  by (induction p; auto)
+
 
 lemma path_h :
   assumes "path M q p"
@@ -120,7 +138,7 @@ lemma path_h :
 
 (* Example FSM *)
 definition "M_ex = (\<lparr> 
-                      initial = 2, 
+                      initial = 2::nat, 
                       inputs = [0,1,2], 
                       outputs = [10,20,30], 
                       transitions = [ (2,1,20,3),
@@ -129,6 +147,17 @@ definition "M_ex = (\<lparr>
                                       (4,0,10,3),
                                       (4,2,20,2),
                                       (5,2,30,3)]\<rparr>)"
+
+definition "M_ex' = (\<lparr> 
+                      initial = 1000::nat, 
+                      inputs = [0,1,2], 
+                      outputs = [10,20,30], 
+                      transitions = [ (1000,1,20,1003),
+                                      (1000,1,30,1003),
+                                      (1003,2,10,1005),
+                                      (1003,0,10,1004),
+                                      (1003,2,20,1002),
+                                      (1005,2,30,1004)]\<rparr>)"
 
 value "nodes M_ex"
 value "path M_ex 2 []"
@@ -185,7 +214,7 @@ qed
 
 value "lists_of_length [1,2,3::nat] 3"
 
-fun paths_of_length :: "FSM \<Rightarrow> State \<Rightarrow> nat \<Rightarrow> Transition list list" where
+fun paths_of_length :: "'state FSM \<Rightarrow> 'state \<Rightarrow> nat \<Rightarrow> 'state Transition list list" where
   "paths_of_length M q n = filter (path M q) (lists_of_length (wf_transitions M) n)"
 
 value "paths M_ex 2 5"
@@ -194,8 +223,8 @@ lemma paths_of_length_containment :
   assumes "path M q p"
   shows "p \<in> set (paths_of_length M q (length p))"
 proof -
-  have "set p \<subseteq> h M" 
-    using assms path_h by auto
+  have "set p \<subseteq> h M"
+    by (meson assms path_h) 
   then have "p \<in> set (lists_of_length (wf_transitions M) (length p))"
     by (metis lists_of_length_containment)
   then show ?thesis
@@ -214,14 +243,14 @@ proof -
 qed
 
 
-fun language_state_for_input :: "FSM \<Rightarrow> State \<Rightarrow> Input list \<Rightarrow> (Input \<times> Output) list list" where
-  "language_state_for_input M q xs = map (map (\<lambda> t . (t_input t, t_output t))) (filter (\<lambda> ts . xs = map t_input ts) (paths_of_length M q (length xs)))"
+fun language_state_for_input :: "'state FSM \<Rightarrow> 'state \<Rightarrow> Input list \<Rightarrow> (Input \<times> Output) list list" where
+  "language_state_for_input M q xs = map p_io (filter (\<lambda> ts . xs = map t_input ts) (paths_of_length M q (length xs)))"
 
 value "language_state_for_input M_ex 2 [1]"
 value "language_state_for_input M_ex 2 [1,2]"
 value "language_state_for_input M_ex 3 [1,2,1,2,1,2]"
 
-fun language_state_for_inputs :: "FSM \<Rightarrow> State \<Rightarrow> Input list list \<Rightarrow> (Input \<times> Output) list list" where
+fun language_state_for_inputs :: "'state FSM \<Rightarrow> 'state \<Rightarrow> Input list list \<Rightarrow> (Input \<times> Output) list list" where
   "language_state_for_inputs M q xss = concat (map (language_state_for_input M q) xss)" 
 
 value "language_state_for_inputs M_ex 2 [[1]]"
@@ -268,8 +297,11 @@ lemma language_state_for_inputs_from_language_state_for_input :
 
 
 
-fun LS\<^sub>i\<^sub>n :: "FSM \<Rightarrow> State \<Rightarrow> Input list set \<Rightarrow> (Input \<times> Output) list set" where 
+fun LS\<^sub>i\<^sub>n :: "'state FSM \<Rightarrow> 'state \<Rightarrow> Input list set \<Rightarrow> (Input \<times> Output) list set" where 
   "LS\<^sub>i\<^sub>n M q U = { map (\<lambda> t . (t_input t, t_output t)) p | p . path M q p \<and> map t_input p \<in> U }"
+
+abbreviation "L\<^sub>i\<^sub>n M \<equiv> LS\<^sub>i\<^sub>n M (initial M)"
+
 
 
 lemma set_map_subset :
@@ -287,7 +319,7 @@ proof
                 and   "x = map (\<lambda> t . (t_input t, t_output t)) p"
     by auto
   have "p \<in> set (filter (\<lambda> ts . map t_input p = map t_input ts) (paths_of_length M q (length (map t_input p))))"
-    using \<open>path M q p\<close> paths_of_length_containment by auto
+    using \<open>path M q p\<close> paths_of_length_containment by fastforce
   then have "map (\<lambda> t . (t_input t, t_output t)) p \<in> set (language_state_for_input M q (map t_input p))"
     by auto
   then obtain tr where  "tr \<in> set (map (language_state_for_input M q) [map t_input p])" 
@@ -345,9 +377,9 @@ proof
   moreover have "map t_input p = map fst x"
     by (simp add: \<open>x = map (\<lambda>t. (t_input t, t_output t)) p\<close>)
   ultimately have "x \<in> LS\<^sub>i\<^sub>n M q {map fst x}"
-    using LS\<^sub>i\<^sub>n.simps \<open>x = map (\<lambda>t. (t_input t, t_output t)) p\<close> by blast  
+    using LS\<^sub>i\<^sub>n.simps \<open>x = map (\<lambda>t. (t_input t, t_output t)) p\<close> by auto 
   moreover have "map fst x \<in> set xss"
-    using \<open>x \<in> set (language_state_for_inputs M q xss)\<close> language_state_for_inputs_inputs by blast
+    using \<open>x \<in> set (language_state_for_inputs M q xss)\<close> language_state_for_inputs_inputs by fastforce
   ultimately show "x \<in> LS\<^sub>i\<^sub>n M q (set xss)"
     using \<open>x = map (\<lambda>t. (t_input t, t_output t)) p\<close> by auto  
 qed
@@ -355,10 +387,253 @@ qed
 
     
 
-lemma LS\<^sub>i\<^sub>n_code[code] : "LS\<^sub>i\<^sub>n M q (set xss) = set (language_state_for_inputs M q xss)" 
-  using LS\<^sub>i\<^sub>n_subset_language_state_for_inputs language_state_for_inputs_subset_LS\<^sub>i\<^sub>n by blast
+lemma LS\<^sub>i\<^sub>n_code[code] : "LS\<^sub>i\<^sub>n M q (set xss) = set (language_state_for_inputs M q xss)"
+  by (meson LS\<^sub>i\<^sub>n_subset_language_state_for_inputs language_state_for_inputs_subset_LS\<^sub>i\<^sub>n subset_antisym) 
+ 
 
 value "LS\<^sub>i\<^sub>n M_ex 2 {[1]}"
 
+
+fun visited_states :: "'state \<Rightarrow> 'state Transition list \<Rightarrow> 'state list" where
+  "visited_states q p = (q # map t_target p)"
+
+fun target :: "'state Transition list \<Rightarrow> 'state \<Rightarrow> 'state" where
+  "target p q = last (visited_states q p)"
+
+
+
+lemma path_append[intro!] :
+  assumes "path M q p1"
+      and "path M (target p1 q) p2"
+  shows "path M q (p1@p2)"
+using assms by (induct p1 arbitrary: p2; auto)
+  
+lemma path_prefix :
+  assumes "path M q (p1@p2)"
+  shows "path M q p1"
+  using assms by (induction p1 arbitrary: q; auto)
+
+lemma path_suffix :
+  assumes "path M q (p1@p2)"
+  shows "path M (target p1 q) p2"
+using assms by (induction p1 arbitrary: q; auto)
+
+lemma path_append_elim[elim!] :
+  assumes "path M q (p1@p2)"
+  obtains "path M q p1"
+      and "path M (target p1 q) p2"
+  by (meson assms path_prefix path_suffix)
+
+
+
+
+
+
+fun LS :: "'state FSM \<Rightarrow> 'state \<Rightarrow> (Input \<times> Output) list set" where
+  "LS M q = { p_io p | p . path M q p }"
+
+abbreviation "L M \<equiv> LS M (initial M)"
+
+
+
+fun cartesian_product_list :: "'a list \<Rightarrow> 'b list \<Rightarrow> ('a \<times> 'b) list" where 
+  "cartesian_product_list xs ys = concat (map (\<lambda> x . map (\<lambda> y . (x,y)) ys) xs)"
+
+value "cartesian_product_list [1,2,3::nat] [10,20,30::nat]"
+
+lemma cartesian_product_list_set : "set (cartesian_product_list xs ys) = {(x,y) | x y . x \<in> set xs \<and> y \<in> set ys}"
+  by auto
+
+fun product_transitions :: "'state1 FSM \<Rightarrow> 'state2 FSM \<Rightarrow> ('state1 \<times> 'state2) Transition list" where
+  "product_transitions A B = map (\<lambda> (t1,t2). ((t_source t1, t_source t2),t_input t1,t_output t1,(t_target t1,t_target t2))) (filter (\<lambda> (t1,t2) . t_input t1 = t_input t2 \<and> t_output t1 = t_output t2) (cartesian_product_list (wf_transitions A) (wf_transitions B)))"
+
+
+value "product_transitions M_ex M_ex'"
+
+
+
+
+
+    
+
+lemma product_transitions_alt1 : "set (product_transitions A B) = {((t_source t1, t_source t2),t_input t1,t_output t1,(t_target t1, t_target t2)) | t1 t2 . (t1,t2) \<in> set (cartesian_product_list (wf_transitions A) (wf_transitions B)) \<and> t_input t1 = t_input t2 \<and> t_output t1 = t_output t2}"
+proof 
+  show "set (product_transitions A B) \<subseteq> {((t_source t1, t_source t2),t_input t1,t_output t1,(t_target t1, t_target t2)) | t1 t2 . (t1,t2) \<in> set (cartesian_product_list (wf_transitions A) (wf_transitions B)) \<and> t_input t1 = t_input t2 \<and> t_output t1 = t_output t2}"
+  proof 
+    fix x assume "x \<in> set (product_transitions A B)"
+    then obtain t1 t2 where "x = ((t_source t1, t_source t2),t_input t1,t_output t1,(t_target t1,t_target t2))"
+                        and "t_input t1 = t_input t2 \<and> t_output t1 = t_output t2"
+                        and "(t1,t2) \<in> set (cartesian_product_list (wf_transitions A) (wf_transitions B))"
+      by force
+    then show "x \<in> {((t_source t1, t_source t2),t_input t1,t_output t1,(t_target t1, t_target t2)) | t1 t2 . (t1,t2) \<in> set (cartesian_product_list (wf_transitions A) (wf_transitions B)) \<and> t_input t1 = t_input t2 \<and> t_output t1 = t_output t2}" by blast
+  qed
+
+  show "{((t_source t1, t_source t2),t_input t1,t_output t1,(t_target t1, t_target t2)) | t1 t2 . (t1,t2) \<in> set (cartesian_product_list (wf_transitions A) (wf_transitions B)) \<and> t_input t1 = t_input t2 \<and> t_output t1 = t_output t2} \<subseteq> set (product_transitions A B)"
+    by force
+qed
+
+lemma product_transitions_alt2 : "set (product_transitions A B) = {((t_source t1, t_source t2),t_input t1,t_output t1,(t_target t1, t_target t2)) | t1 t2 . t1 \<in> set (wf_transitions A) \<and> t2 \<in> set (wf_transitions B) \<and> t_input t1 = t_input t2 \<and> t_output t1 = t_output t2}"
+(is "?P = ?A2")
+proof -
+  have "?P = {((t_source t1, t_source t2),t_input t1,t_output t1,(t_target t1, t_target t2)) | t1 t2 . (t1,t2) \<in> set (cartesian_product_list (wf_transitions A) (wf_transitions B)) \<and> t_input t1 = t_input t2 \<and> t_output t1 = t_output t2}"
+    using product_transitions_alt1 by assumption
+  also have "... = ?A2" by force
+  finally show ?thesis by auto
+qed
+
+lemma product_transitions_alt3 : "set (product_transitions A B) = {((q1,q2),x,y,(q1',q2')) | q1 q2 x y q1' q2' . (q1,x,y,q1') \<in> set (wf_transitions A) \<and> (q2,x,y,q2') \<in> set (wf_transitions B)}"
+(is "?P = ?A3")
+proof -
+  have "?P = {((t_source t1, t_source t2),t_input t1,t_output t1,(t_target t1, t_target t2)) | t1 t2 . t1 \<in> set (wf_transitions A) \<and> t2 \<in> set (wf_transitions B) \<and> t_input t1 = t_input t2 \<and> t_output t1 = t_output t2}"
+    using product_transitions_alt2 by assumption
+  also have "... = ?A3" by force
+  finally show ?thesis by simp
+qed
+
+
+definition product :: "'state1 FSM \<Rightarrow> 'state2 FSM \<Rightarrow> ('state1 \<times> 'state2) FSM" where
+  "product A B \<equiv>
+  \<lparr>
+    initial = (initial A, initial B),
+    inputs = (inputs A) @ (inputs B),
+    outputs = (outputs A) @ (outputs B),
+    transitions = product_transitions A B    
+  \<rparr>"
+
+    (*
+    inputs = remdups ((inputs A) @ (inputs B)),
+    outputs = remdups ((outputs A) @ (outputs B)),
+    transitions = remdups (product_transitions A B)
+    *)
+
+
+value "product M_ex M_ex'"
+
+lemma product_simps[simp]:
+  "initial (product A B) = (initial A, initial B)"  
+  "inputs (product A B) = inputs A @ inputs B"
+  "outputs (product A B) = outputs A @ outputs B"
+  "transitions (product A B) = product_transitions A B"
+unfolding product_def by simp+
+
+lemma product_path[iff]:
+  "path (product A B) (q1,q2) p \<longleftrightarrow> (path A q1 (map (\<lambda> t . (fst (t_source t), t_input t, t_output t, fst (t_target t))) p)
+                                            \<and> path B q2 (map (\<lambda> t . (snd (t_source t), t_input t, t_output t, snd (t_target t))) p))"
+proof (induction p arbitrary: q1 q2)
+case Nil
+then show ?case by auto
+next
+  case (Cons t p)
+  then show ?case 
+  proof (cases "path (product A B) (q1, q2) [t]")
+    case True
+    then have "t \<in> h (product A B)"
+      by (meson path'.simps(2) path_code) 
+    then obtain t1 t2 where "t = ((t_source t1, t_source t2),t_input t1,t_output t1,(t_target t1, t_target t2))"
+                        and "t1 \<in> set (wf_transitions A)" 
+                        and "t2 \<in> set (wf_transitions B)" 
+                        and "t_input t1 = t_input t2 \<and> t_output t1 = t_output t2"
+    proof -
+      assume a1: "\<And>t1 t2. \<lbrakk>t = ((t_source t1, t_source t2), t_input t1, t_output t1, t_target t1, t_target t2); t1 \<in> h A; t2 \<in> h B; t_input t1 = t_input t2 \<and> t_output t1 = t_output t2\<rbrakk> \<Longrightarrow> thesis"
+      have "(q1, q2) = t_source t \<and> path (product A B) (t_target t) [] \<and> t \<in> set (transitions (product A B)) \<and> t_input t \<in> set (inputs (product A B)) \<and> t_output t \<in> set (outputs (product A B))"
+        using True by blast
+      then have "t \<in> {((t_source p, t_source pa), t_input p, t_output p, t_target p, t_target pa) | p pa. p \<in> h A \<and> pa \<in> h B \<and> t_input p = t_input pa \<and> t_output p = t_output pa}"
+        by (metis product_simps(4) product_transitions_alt2)
+      then show ?thesis
+        using a1 by blast
+    qed
+
+    have "t1 = (fst (t_source t), t_input t, t_output t, fst (t_target t))" 
+      using \<open>t = ((t_source t1, t_source t2),t_input t1,t_output t1,(t_target t1, t_target t2))\<close> by auto
+    then have "(fst (t_source t), t_input t, t_output t, fst (t_target t)) \<in> h A"
+      using \<open>t1 \<in> set (wf_transitions A)\<close> by auto
+    have "path A q1 [(fst (t_source t), t_input t, t_output t, fst (t_target t))]"
+    proof -
+      have "q1 = t_source (fst (t_source t), t_input t, t_output t, fst (t_target t))"
+        by (metis (no_types) True fst_conv path'.simps(2) path_code)
+      then show ?thesis
+        using \<open>(fst (t_source t), t_input t, t_output t, fst (t_target t)) \<in> h A\<close> by blast
+    qed
+
+    then have *: "path A q1 (map (\<lambda>t. (fst (t_source t), t_input t, t_output t, fst (t_target t))) (t # p)) = path A (fst (t_target t)) (map (\<lambda>t. (fst (t_source t), t_input t, t_output t, fst (t_target t))) p)"
+      by auto
+
+    have "t2 = (snd (t_source t), t_input t, t_output t, snd (t_target t))" 
+      using \<open>t = ((t_source t1, t_source t2),t_input t1,t_output t1,(t_target t1, t_target t2))\<close> \<open>t_input t1 = t_input t2 \<and> t_output t1 = t_output t2\<close> by auto
+    then have "(snd (t_source t), t_input t, t_output t, snd (t_target t)) \<in> h B"
+      using \<open>t2 \<in> set (wf_transitions B)\<close> by auto
+    have "path B q2 [(snd (t_source t), t_input t, t_output t, snd (t_target t))]"
+    proof -
+      have "(t_source t1, t_source t2) = (q1, q2)"
+        by (metis (no_types) True \<open>t = ((t_source t1, t_source t2), t_input t1, t_output t1, t_target t1, t_target t2)\<close> fstI path'.simps(2) path_code)
+      then have "t_source t1 = q1 \<and> t_source t2 = q2"
+        by simp
+      then show ?thesis
+        using \<open>(snd (t_source t), t_input t, t_output t, snd (t_target t)) \<in> h B\<close> \<open>t2 = (snd (t_source t), t_input t, t_output t, snd (t_target t))\<close> by fastforce
+    qed
+
+    then have **: "path B q2 (map (\<lambda>t. (snd (t_source t), t_input t, t_output t, snd (t_target t))) (t # p)) = path B (snd (t_target t)) (map (\<lambda>t. (snd (t_source t), t_input t, t_output t, snd (t_target t))) p)"
+      by auto
+
+    have ***: "path (product A B) (q1, q2) (t # p) = path (product A B) (t_target t) p"
+      by (metis True path'.simps(2) path_code) 
+      
+      
+
+    show ?thesis
+      by (metis (no_types, lifting) "*" "**" Cons.IH "***" prod.collapse)
+  next
+    case False
+    then have *: "\<not> path (product A B) (q1, q2) (t # p)"
+      by (metis (no_types, lifting) list.distinct(1) list.sel(1) path.simps) 
+
+    have "\<not> (path A q1 [(fst (t_source t), t_input t, t_output t, fst (t_target t))]
+              \<and> path B q2 [(snd (t_source t), t_input t, t_output t, snd (t_target t))])"
+    proof (rule ccontr)
+      assume "\<not> \<not> (path A q1 [(fst (t_source t), t_input t, t_output t, fst (t_target t))]
+              \<and> path B q2 [(snd (t_source t), t_input t, t_output t, snd (t_target t))])"
+      then have "q1 = fst (t_source t)"
+           and  "q2 = snd (t_source t)"
+           and  "(fst (t_source t), t_input t, t_output t, fst (t_target t)) \<in> h A"
+           and  "(snd (t_source t), t_input t, t_output t, snd (t_target t)) \<in> h B"
+        by auto
+
+      have "t \<in> set (transitions (product A B))"
+      proof -
+        have "t = ((fst (t_source t), snd (t_source t)), t_input t, t_output t, fst (t_target t), snd (t_target t))"
+          by auto
+        then have "t \<in> {((a, b), n, na, aa, ba) |a b n na aa ba. (a, n, na, aa) \<in> h A \<and> (b, n, na, ba) \<in> h B}"
+          using \<open>(fst (t_source t), t_input t, t_output t, fst (t_target t)) \<in> h A\<close> \<open>(snd (t_source t), t_input t, t_output t, snd (t_target t)) \<in> h B\<close> by blast
+        then show ?thesis
+          by (metis (no_types) product_simps(4) product_transitions_alt3)
+      qed 
+
+      have "t_input t \<in> set (inputs A)" 
+      and  "t_output t \<in> set (outputs A)"
+        using \<open>(fst (t_source t), t_input t, t_output t, fst (t_target t)) \<in> h A\<close> by auto
+      then have "t_input t \<in> set (inputs (product A B))" 
+           and  "t_output t \<in> set (outputs (product A B))" 
+        by auto
+
+      have "t \<in> h (product A B)"
+        by (metis \<open>t \<in> set (transitions (product A B))\<close> \<open>t_input t \<in> set (inputs (product A B))\<close> \<open>t_output t \<in> set (outputs (product A B))\<close> filter_set is_wf_transition.elims(3) member_filter wf_transitions.elims) 
+        
+      have "path (product A B) (q1, q2) [t]"
+        by (metis \<open>q1 = fst (t_source t)\<close> \<open>q2 = snd (t_source t)\<close> \<open>t \<in> h (product A B)\<close> path.simps prod.collapse)
+        
+      then show "False" using False by auto 
+    qed
+
+    then have **: "\<not> (path A q1 (map (\<lambda>t. (fst (t_source t), t_input t, t_output t, fst (t_target t))) (t # p)) 
+                      \<and> path B q2 (map (\<lambda>t. (snd (t_source t), t_input t, t_output t, snd (t_target t))) (t # p)))" by auto
+
+    show ?thesis using * ** by auto
+  qed
+qed
+
+
+
+lemma "LS (product A B) (q1,q2) = LS A q1 \<inter> LS B q2"
+  unfolding LS.simps using product_path[of A B q1 q2] sorry
 
 end
